lib/ListSupport.v
@@ -1,0 +1,180 @@
+Require Import Coq.Lists.List Lib.Concat.
+
+Import ListNotations.
+
+Set Implicit Arguments.
+
+Lemma hd_error_revcons_same A ls: forall (a: A), hd_error ls = Some a ->
+                                                 forall v, hd_error (ls ++ [v]) = Some a.
+Proof.
+  induction ls; auto; simpl; intros; discriminate.
+Qed.
+
+Lemma hd_error_revcons_holds A (P: A -> Prop) (ls: list A):
+  forall a, hd_error ls = Some a ->
+            P a ->
+            forall b v, hd_error (ls ++ [v]) = Some b ->
+                        P b.
+Proof.
+  intros.
+  rewrite hd_error_revcons_same with (a := a) in H1; auto.
+  inversion H1; subst; auto.
+Qed.
+
+Lemma single_unfold_concat A B a (f: A -> list B) (ls: list A):
+  concat (map f (a :: ls)) = (f a ++ concat (map f ls))%list.
+Proof.
+  reflexivity.
+Qed.
+
+Lemma in_single: forall A (a l: A), In a (l :: nil) -> a = l.
+Proof.
+  intros.
+  simpl in *.
+  destruct H; intuition auto.
+Qed.
+
+Lemma in_pre_suf: forall A l (a: A), In a l -> exists l1 l2, (l = l1 ++ a :: l2)%list.
+Proof.
+  induction l; simpl.
+  - intuition auto.
+  - intros.
+    destruct H; [| apply IHl in H; intuition auto].
+    + subst.
+      exists nil, l.
+      reflexivity.
+    + destruct H as [? [? ?]].
+      subst.
+      exists (a :: x), x0.
+      reflexivity.
+Qed.
+
+Lemma list_nil_revcons A: forall (l: list A), l = nil \/ exists l' v, l = (l' ++ [v])%list.
+Proof.
+  induction l; subst.
+  - left; auto.
+  - destruct IHl; subst.
+    + right.
+      exists nil, a.
+      reflexivity.
+    + destruct H as [? [? ?]];
+      subst.
+      right; simpl.
+      exists (a :: x), x0.
+      reflexivity.
+Qed.
+
+
+Lemma app_single_r: forall A (ls1 ls2: list A) v1 v2,
+                      (ls1 ++ [v1] = ls2 ++ [v2])%list ->
+                      ls1 = ls2 /\ v1 = v2.
+Proof.
+  induction ls1; simpl; auto; intros.
+  - destruct ls2; simpl in *; inversion H; auto.
+    apply app_cons_not_nil in H2.
+    intuition auto.
+  - destruct ls2; simpl in *; inversion H; auto.
+    + apply eq_sym in H2; apply app_cons_not_nil in H2.
+      intuition auto.
+    + specialize (IHls1 _ _ _ H2).
+      intuition (try f_equal; auto).
+Qed.
+
+Lemma app_cons_in A ls:
+  forall (v: A) s1 s2 beg mid last,
+    (ls ++ [v] = beg ++ s1 :: mid ++ s2 :: last)%list ->
+    In s1 ls.
+Proof.
+  induction ls; simpl; auto; intros;
+  destruct beg; simpl in *; inversion H.
+  - apply app_cons_not_nil in H2.
+    auto.
+  - apply app_cons_not_nil in H2.
+    auto.
+  - intuition auto.
+  - apply IHls in H2; intuition auto.
+Qed.
+
+Lemma beg_mid_last_add_eq A ls:
+  (forall (v: A) v1 v2 beg mid last,
+     ls ++ [v] = beg ++ v1 :: mid ++ v2 :: last ->
+     (last = nil /\ v = v2 /\ ls = beg ++ v1 :: mid) \/
+     (exists last', last = last' ++ [v] /\ ls = beg ++ v1 :: mid ++ v2 :: last'))%list.
+Proof.
+  intros.
+  pose proof (list_nil_revcons last) as [sth1 | sth2].
+  - subst.
+    left.
+    rewrite app_comm_cons in H.
+    rewrite app_assoc in H.
+    apply app_single_r in H.
+    destruct H as [? ?].
+    repeat (constructor; auto).
+  - destruct sth2 as [? [? ?]].
+    right.
+    exists x.
+    subst.
+    rewrite app_comm_cons in H.
+    rewrite app_assoc in H.
+    rewrite app_comm_cons in H.
+    rewrite app_assoc in H.
+    apply app_single_r in H.
+    destruct H as [? ?]; subst.
+    repeat (constructor; auto).
+    rewrite app_comm_cons.
+    rewrite app_assoc.
+    reflexivity.
+Qed.
+
+Lemma in_revcons A ls (a v: A):
+  In v (ls ++ (a :: nil)) ->
+  In v ls \/ v = a.
+Proof.
+  intros.
+  apply in_app_or in H.
+  simpl in *.
+  intuition.
+Qed.
+
+Lemma in_cons A ls (a v: A):
+  In v (a :: ls) ->
+  In v ls \/ v = a.
+Proof.
+  simpl.
+  intuition.
+Qed.
+
+Lemma in_revcons_converse A ls (a v: A):
+  In v ls \/ v = a ->
+  In v (ls ++ (a :: nil)).
+Proof.
+  intros.
+  apply in_or_app.
+  simpl in *.
+  intuition.
+Qed.
+
+Lemma in_cons_converse A ls (a v: A):
+  In v ls \/ v = a ->
+  In v (a :: ls).
+Proof.
+  simpl.
+  intuition.
+Qed.
+
+Ltac destruct_in :=
+  repeat match goal with
+           | H: In ?v (?ls ++ ?a :: nil) |- _ =>
+             apply (in_revcons ls a v) in H;
+               let isEq := fresh in
+               (destruct H as [ ? | isEq]; [| rewrite isEq in *])
+           | H: In ?v (?a :: ?ls) |- _ =>
+             apply (in_cons) in H;
+               let isEq := fresh in
+               (destruct H as [ ? | isEq]; [| rewrite isEq in *])
+           | |- In ?v (?ls ++ ?a :: nil) =>
+             apply (in_revcons_converse ls)
+           | |- In ?v (?a :: ?ls) =>
+             apply (in_cons_converse ls)
+         end.
+      
