lib/Misc.v
@@ -1,0 +1,48 @@
+Require Import String StringExtension.
+
+Open Scope string.
+
+Set Implicit Arguments.
+
+Theorem true_False_false: forall v, (v = true -> False) -> v = false.
+Proof.
+  intros.
+  destruct v; intuition auto.
+Qed.
+
+Theorem false_False_true: forall v, (v = false -> False) -> v = true.
+Proof.
+  intros.
+  destruct v; intuition auto.
+Qed.
+
+Ltac simplBool :=
+  match goal with
+    | H: ?v = true -> False |- _ =>
+      apply true_False_false in H
+    | H: ?v = false -> False |- _ =>
+      apply false_False_true in H
+  end.
+
+Lemma not_in_string_uneq':
+  forall a x n s, ~ S_In a s -> s <> x ++ (String a n).
+Proof.
+  induction x; simpl; auto; intros; intro; subst; simpl in *; [intuition auto|].
+  assert (sth: ~ S_In a (x ++ String a n)) by intuition auto.
+  clear - sth.
+  assert ((S_In a x \/ S_In a (String a n)) -> False) by
+      (intros H; apply S_in_or_app in H; intuition auto).
+  assert (sth2: S_In a (String a n) -> False) by intuition auto.
+  simpl in sth2.
+  intuition auto.
+Qed.
+
+Lemma not_in_string_uneq:
+  forall a x n s, index 0 (String a EmptyString) s = None -> s <> x ++ (String a n).
+Proof.
+  intros.
+  apply not_in_string_uneq'.
+  apply index_not_in; auto.
+Qed.
+
+Close Scope string.
